BackTrans/InjectExtract.v
@@ -1,0 +1,106 @@
+Require Stlc.SpecSyntax.
+Require Utlc.SpecSyntax.
+Require Import Stlc.SpecTyping.
+Require Import Stlc.LemmasTyping.
+Require Import Stlc.SpecEvaluation.
+Require Import Stlc.LemmasEvaluation.
+Require Import Stlc.StlcOmega.
+Require Import Utlc.SpecScoping.
+Require Import Utlc.LemmasScoping.
+Require Import Utlc.DecideEval.
+Require Import LogRel.PseudoType.
+Require Import LogRel.LemmasPseudoType.
+Require Import LogRel.LR.
+Require Import LogRel.LemmasLR.
+Require Import LogRel.LemmasIntro.
+Require Import Omega.
+Require Import Db.Lemmas.
+
+
+Require Import LogRel.LR.
+Require Import Compiler.ProtectConfine.
+
+Require Import BackTrans.UValHelpers.
+
+Require Import UVal.UVal.
+
+Fixpoint inject (n : nat) (τ : Ty) :=
+  S.abs τ
+      (match τ with
+         | tarr τ₁ τ₂ => inArrDwn n (S.abs (UVal n) (S.app (inject n τ₂) (S.app (S.var 1) (S.app (extract n τ₁) (S.var 0)))))
+         | tunit => inUnitDwn n (S.var 0) 
+         | tbool => inBoolDwn n (S.var 0)
+         | tprod τ₁ τ₂ => inProdDwn n (S.pair (S.app (inject n τ₁) (S.proj₁ (S.var 0))) 
+                                         (S.app (inject n τ₂) (S.proj₂ (S.var 0))))
+         | tsum τ₁ τ₂ => inSumDwn n (S.caseof (S.var 0) (S.inl (S.app (inject n τ₁) (S.var 0))) 
+                                         (S.inr (S.app (inject n τ₂) (S.var 0))))
+       end)
+with extract (n : nat) (τ : Ty) :=
+       S.abs (UVal n) (match τ with
+                       | tarr τ₁ τ₂ => S.abs τ₁ (S.app (extract n τ₂) (S.app (caseArrUp n (S.var 1)) (S.app (inject n τ₁) (S.var 0))))
+                       | tunit => caseUnitUp n (S.var 0)
+                       | tbool => caseBoolUp n (S.var 0)
+                       | tprod τ₁ τ₂ => S.pair (S.app (extract n τ₁) (S.proj₁ (caseProdUp n (S.var 0))))
+                                             (S.app (extract n τ₂) (S.proj₂ (caseProdUp n (S.var 0))))
+                       | tsum τ₁ τ₂ => S.caseof (caseSumUp n (S.var 0))
+                                              (S.inl (S.app (extract n τ₁) (S.var 0)))
+                                              (S.inr (S.app (extract n τ₂) (S.var 0)))
+                     end).
+
+
+Lemma injectT {n τ Γ} : ⟪ Γ ⊢ inject n τ : τ ⇒ UVal n ⟫
+with extractT {n τ Γ} : ⟪ Γ ⊢ extract n τ : UVal n ⇒ τ ⟫. 
+Proof.
+  - induction τ; unfold inject; eauto with typing uval_typing.
+  - induction τ; unfold extract; eauto with typing uval_typing.
+Qed.
+
+Lemma inject_closed {n τ} :
+  ⟨ 0 ⊢ inject n τ ⟩.
+Proof.
+  eapply (wt_implies_ws (Γ := empty)).
+  eapply injectT.
+Qed.
+
+Lemma extract_closed {n τ} :
+  ⟨ 0 ⊢ extract n τ ⟩.
+Proof.
+  eapply (wt_implies_ws (Γ := empty)).
+  eapply extractT.
+Qed.
+
+Lemma inject_sub {n τ γ} : (inject n τ)[γ] = inject n τ.
+Proof.
+  apply wsClosed_invariant.
+  eapply inject_closed.
+Qed.
+
+Lemma extract_sub {n τ γ} : (extract n τ)[γ] = extract n τ.
+Proof.
+  apply wsClosed_invariant.
+  eapply extract_closed.
+Qed.
+
+Lemma inject_and_protect_work {n w d p τ vs vu} :
+  dir_world_prec n w d p →
+  valrel d w (embed τ) vs vu →
+  termrel₀ d w (pEmulDV n p) (S.app (inject n τ) vs) (U.app (protect τ) vu).
+Proof.
+  revert n w vs vu.
+  induction τ;
+  intros n w vs vu dwp vr; simpl.
+  - (* τ₁ ⇒ τ₂ *) 
+    destruct (valrel_implies_Value vr) as (vvs & vvu).
+    eapply termrel₀_antired_star.
+    + eapply evalToStar.
+      eapply (S.eval_ctx₀ S.phole); simpl;
+      eauto using S.eval_beta.
+    + eapply evalToStar.
+      eapply U.eval₀_ctxeval.
+      eapply U.eval_beta; eauto.
+    + cbn.
+      rewrite inArrDwn_sub, protect_sub, confine_sub. 
+      crushTyping.
+      rewrite inject_sub, extract_sub; cbn.
+      crushUtlcScoping.
+      rewrite protect_sub, confine_sub.
